src/HOL/Theorie.v
@@ -1,583 +1,110 @@
-From CRM Require Import Base Typing Reduction fintype.
-Import CombineNotations SubstNotations.
-
-Require Import PeanoNat List Datatypes Program.Equality.
+Require Import Base.
+From Stdlib Require Import List.
 Import ListNotations.
+From Stdlib Require Import Program.Equality.
 
-(*Reserved Notation "Γ | Ξ ⊢⟨ n ⟩ φ" (at level 88).*)
+Definition proof_ctx (Γ : HOL_ctx) : Type := list (Γ ⊢ₛ ℙₛ).
 
+(* Standardity predicate are defined inductively :
+ℕ(x) ≜ ∀ X : ℕ → ℙ, X 0 ⇒ (∀ n : ℕ, X n ⇒ X (n + 1)) ⇒ X x
+𝔹(x) ≜ ∀ X : 𝔹 → ℙ, X ⊤ ⇒ X ⊥ ⇒ X x
+(𝕃ₛ S)(x) ≜
+  ∀ X : 𝕃ₛ S → ℙ, X [] ⇒ (∀ (s : S) (l : 𝕃ₛ), S(x) ⇒ X l ⇒ X (s :: l)) ⇒ X x
+ℙ(φ) ≜ True
+𝟙(x) ≜ ∀ X : 𝟙 → ℙ, X ⟨⟩ ⇒ X x
+𝟘(x) ≜ ∀ X : 𝟘 → ℙ, X x
+(S → T)(f) ≜ ∀ s : S, S(s) ⇒ T(f x)
+(S × T)(x) ≜ S(π₁ x) ∧ S(π₂ x)
+(S + T)(x) ≜
+  ∀ X : S + T → ℙ, (∀ s : S, X(κ₁ s)) ⇒ (∀ t : T, X(κ₂ t)) ⇒ X x
+*)
 
-Require Import CRM.Prelude.ListCRM.
+Notation vz := (vz_tm _ _).
+Notation vs := (vs_tm _).
 
-Definition proof_ctx (n : nat) := list (tm n).
+Equations Standardity (Γ : HOL_ctx) (s : st) : Γ ⊢ₛ s →ₛ ℙₛ :=
+  Standardity Γ ℕₛ :=
+    ƛₛ ℕₛ
+      (∀ₛ (ℕₛ →ₛ ℙₛ)
+        ((⟦ vz ⟧ₛ @ₛ 0ₛ) ⇒ₛ
+           (∀ₛ ℕₛ (⟦ vs vz ⟧ₛ @ₛ ⟦ vz ⟧ₛ ⇒ₛ ⟦ vs vz ⟧ₛ @ₛ Sₛ ⟦ vz ⟧ₛ)) ⇒ₛ
+           ⟦ vz ⟧ₛ @ₛ ⟦ vs vz ⟧ₛ)) ;
+  Standardity Γ 𝔹ₛ :=
+    ƛₛ 𝔹ₛ
+      (∀ₛ (𝔹ₛ →ₛ ℙₛ)
+        ((⟦ vz ⟧ₛ @ₛ ⊤ₛ) ⇒ₛ (⟦ vz ⟧ₛ @ₛ ⊥ₛ) ⇒ₛ (⟦ vz ⟧ₛ @ₛ ⟦ vs vz ⟧ₛ))) ;
+  Standardity Γ (𝕃ₛ s) :=
+    ƛₛ (𝕃ₛ s)
+      (∀ₛ (𝕃ₛ s →ₛ ℙₛ)
+        ((⟦ vz ⟧ₛ @ₛ []ₛ) ⇒ₛ
+           (∀ₛ s ((Standardity _ s) @ₛ ⟦ vz ⟧ₛ ⇒ₛ
+                    (∀ₛ (𝕃ₛ s)
+                      (⟦ vs (vs vz) ⟧ₛ @ₛ ⟦ vz ⟧ₛ ⇒ₛ
+                         ⟦ vs (vs vz) ⟧ₛ @ₛ (⟦ vs vz ⟧ₛ ::ₛ ⟦ vz ⟧ₛ))))) ⇒ₛ
+           ⟦ vz ⟧ₛ @ₛ ⟦ vs vz ⟧ₛ)) ;
+  Standardity Γ ℙₛ := ƛₛ ℙₛ (∀ₛ ℙₛ (⟦ vz ⟧ₛ ⇒ₛ ⟦ vz ⟧ₛ)) ;
+  Standardity Γ 𝟙ₛ := ƛₛ 𝟙ₛ (∀ₛ (𝟙ₛ →ₛ ℙₛ) (⟦ vz ⟧ₛ @ₛ ⟨⟩ₛ ⇒ₛ ⟦ vz ⟧ₛ @ₛ ⟦ vs vz ⟧ₛ)) ;
+  Standardity Γ 𝟘ₛ := ƛₛ 𝟘ₛ (∀ₛ (𝟘ₛ →ₛ ℙₛ) (⟦ vz ⟧ₛ @ₛ ⟦ vs vz ⟧ₛ)) ;
+  Standardity Γ (s →ₛ t) :=
+    ƛₛ (s →ₛ t) (∀ₛ s (Standardity _ s @ₛ ⟦ vz ⟧ₛ ⇒ₛ
+                        Standardity _ t @ₛ (⟦ vs vz ⟧ₛ @ₛ ⟦ vz ⟧ₛ))) ;
+  Standardity Γ (s ×ₛ t) :=
+    ƛₛ (s ×ₛ t)
+      (∀ₛ (s ×ₛ t →ₛ ℙₛ) (
+           (∀ₛ s (Standardity _ s @ₛ ⟦ vz ⟧ₛ ⇒ₛ
+                  (∀ₛ t (Standardity _ t @ₛ ⟦ vz ⟧ₛ ⇒ₛ
+                          (⟦ vs (vs vz) ⟧ₛ @ₛ ⟨ ⟦ vs vz ⟧ₛ, ⟦ vz ⟧ₛ ⟩ₛ))))) ⇒ₛ
+             ⟦ vz ⟧ₛ @ₛ ⟦ vs vz ⟧ₛ)) ;
+  Standardity Γ (s +ₛ t) :=
+    ƛₛ (s +ₛ t)
+      (∀ₛ (s +ₛ t →ₛ ℙₛ) (
+           (∀ₛ s (Standardity _ s @ₛ ⟦ vz ⟧ₛ ⇒ₛ ⟦ vs vz ⟧ₛ @ₛ κ¹ₛ _ ⟦ vz ⟧ₛ)) ⇒ₛ
+             (∀ₛ t (Standardity _ t @ₛ ⟦ vz ⟧ₛ ⇒ₛ ⟦ vs vz ⟧ₛ @ₛ κ²ₛ _ ⟦ vz ⟧ₛ)) ⇒ₛ
+             ⟦ vz ⟧ₛ @ₛ ⟦ vs vz ⟧ₛ)).
 
-Definition wt_ctx {n : nat} (Γ : HOL_ctx n) (Ξ : proof_ctx n) : Type :=
-  forall_l (fun Θ => Γ ⊢⟨ n ⟩ Θ ~: ℙₛ) Ξ.
+Inductive proof : forall (Γ : HOL_ctx), proof_ctx Γ -> Γ ⊢ₛ ℙₛ -> Prop :=
+| pr_ax : forall {Γ : HOL_ctx} {Ξ : proof_ctx Γ} {φ : Γ ⊢ₛ ℙₛ},
+    In φ Ξ -> proof Γ Ξ φ
+| pr_imp_i : forall {Γ : HOL_ctx} {Ξ : proof_ctx Γ} {φ ψ : Γ ⊢ₛ ℙₛ},
+    proof Γ (φ :: Ξ) ψ -> proof Γ Ξ (φ ⇒ₛ ψ)
+| pr_imp_e : forall {Γ : HOL_ctx} {Ξ : proof_ctx Γ} (φ : Γ ⊢ₛ ℙₛ) {ψ : Γ ⊢ₛ ℙₛ},
+    proof Γ Ξ (φ ⇒ₛ ψ) -> proof Γ Ξ φ -> proof Γ Ξ ψ
+| pr_fora_i : forall {Γ : HOL_ctx} {s : st} {Ξ : proof_ctx Γ}
+                     {φ : s :: Γ ⊢ₛ ℙₛ},
+    proof (s :: Γ) (map (fun φ => φ ↑ₛ s) Ξ) φ -> proof Γ Ξ (∀ₛ s φ)
+| pr_fora_e : forall {Γ : HOL_ctx} {s : st} {Ξ : proof_ctx Γ}
+                     {φ : s :: Γ ⊢ₛ ℙₛ} (t : Γ ⊢ₛ s),
+    proof Γ Ξ (∀ₛ s φ) -> proof Γ Ξ (φ ⟨[ t ::ᵥ id_subst Γ ]⟩)
+| pr_stand : forall {Γ : HOL_ctx} (s : st) {Ξ : proof_ctx Γ},
+    proof Γ Ξ (∀ₛ s (Standardity (s :: Γ) s @ₛ ⟦ vz ⟧ₛ)).
 
-Inductive proving : forall (n : nat) (Γ : HOL_ctx n)
-                           (Ξ : proof_ctx n) (φ : tm n), Prop :=
-| pr_ax : forall {n : nat} {Γ : HOL_ctx n}
-                 {Ξ : proof_ctx n} {φ : tm n},
-    wt_ctx Γ Ξ -> In φ Ξ -> proving n Γ Ξ φ
-| pr_transp : forall {n : nat} {Γ : HOL_ctx n}
-                     {Ξ : proof_ctx n} (φ : tm n)
-                     {ψ : tm n},
-    proving n Γ Ξ φ -> Γ ⊢⟨ n ⟩ ψ ~: ℙₛ ->
-    φ =ₛ ψ -> proving n Γ Ξ ψ
-| pr_abs : forall {n : nat} {Γ : HOL_ctx n}
-                  {Ξ : proof_ctx n} {φ ψ : tm n},
-    proving n Γ (φ :: Ξ) ψ -> proving n Γ Ξ (φ ⇒ₛ ψ)
-| pr_app : forall {n : nat} {Γ : HOL_ctx n}
-                  {Ξ : proof_ctx n} (φ : tm n)
-                  {ψ : tm n},
-    proving n Γ Ξ (φ ⇒ₛ ψ) -> proving n Γ Ξ φ ->
-    proving n Γ Ξ ψ
-| pr_abs_f : forall {n : nat} {Γ : HOL_ctx n} {Ξ : proof_ctx n}
-                    {φ : tm (S n)} {s : st},
-    proving (S n) (s .: Γ) (List.map (ren_tm shift) Ξ) φ ->
-    proving n Γ Ξ (∀ₛ s φ)
-| pr_app_f : forall {n : nat} {Γ : HOL_ctx n} {Ξ : proof_ctx n}
-                    {φ : tm (S n)} (t : tm n) (s : st),
-    proving n Γ Ξ (∀ₛ s φ) -> Γ ⊢⟨ n ⟩ t ~: s ->
-    proving n Γ Ξ (φ [t .: (fun v => ⟦ v ⟧ₛ)])
-| pr_recN : forall {n : nat} {Γ : HOL_ctx n} {Ξ : proof_ctx n}
-                   {φ : tm n},
-    proving n Γ Ξ (φ @ₛ Zₛ) ->
-    proving n Γ Ξ
-      (∀ₛ ℕₛ ((ren_tm shift φ @ₛ ((S n) __tm var_zero)) ⇒ₛ
-                (ren_tm shift φ @ₛ (Sₛ ((S n) __tm var_zero))))) ->
-    proving n Γ Ξ (∀ₛ ℕₛ (ren_tm shift φ @ₛ ((S n) __tm var_zero)))
-| pr_recB : forall {n : nat} {Γ : HOL_ctx n} {Ξ : proof_ctx n}
-                   {φ : tm n},
-    proving n Γ Ξ (φ @ₛ ttₛ) ->
-    proving n Γ Ξ (φ @ₛ ffₛ) ->
-    proving n Γ Ξ (∀ₛ 𝔹ₛ (ren_tm shift φ @ₛ ((S n) __tm var_zero)))
-| pr_recL : forall {n : nat} {Γ : HOL_ctx n} {Ξ : proof_ctx n}
-                   {s : st} {φ : tm n},
-    proving n Γ Ξ (φ @ₛ []ₛ) ->
-    proving n Γ Ξ
-      (∀ₛ s
-        (∀ₛ (𝕃ₛ s)
-          (ren_tm (shift >> shift) φ @ₛ
-             (((S (S n)) __tm (shift var_zero)) ::ₛ
-             ((S (S n)) __tm var_zero))))) ->
-    proving n Γ Ξ (∀ₛ (𝕃ₛ s) (ren_tm shift φ @ₛ ((S n) __tm var_zero)))
-| pr_sort_Z : forall {n : nat} {Γ : HOL_ctx n} {Ξ : proof_ctx n},
-    wt_ctx Γ Ξ -> proving n Γ Ξ (𝕊 ℕₛ Zₛ)
-| pr_sort_S : forall {n : nat} {Γ : HOL_ctx n} {Ξ : proof_ctx n}
-                     {t : tm n},
-    proving n Γ Ξ (𝕊 ℕₛ t) -> proving n Γ Ξ (𝕊 ℕₛ (Sₛ t))
-| pr_sort_recN : forall {n : nat} {Γ : HOL_ctx n} {Ξ : proof_ctx n}
-                        {t u v : tm n} {s : st},
-    proving n Γ Ξ (𝕊 s t) -> proving n Γ Ξ (𝕊 (ℕₛ →ₛ s →ₛ s) u) ->
-    proving n Γ Ξ (𝕊 ℕₛ v) -> proving n Γ Ξ (𝕊 s (recℕₛ t u v))
-| pr_sort_T : forall {n : nat} {Γ : HOL_ctx n} {Ξ : proof_ctx n},
-    wt_ctx Γ Ξ -> proving n Γ Ξ (𝕊 𝔹ₛ ttₛ)
-| pr_sort_F : forall {n : nat} {Γ : HOL_ctx n} {Ξ : proof_ctx n},
-    wt_ctx Γ Ξ -> proving n Γ Ξ (𝕊 𝔹ₛ ffₛ)
-| pr_sort_recB : forall {n : nat} {Γ : HOL_ctx n} {Ξ : proof_ctx n}
-                        {t u v : tm n} {s : st},
-    proving n Γ Ξ (𝕊 s t) -> proving n Γ Ξ (𝕊 s u) ->
-    proving n Γ Ξ (𝕊 𝔹ₛ v) -> proving n Γ Ξ (𝕊 s (rec𝔹ₛ t u v))
-| pr_sort_nil : forall {n : nat} {Γ : HOL_ctx n} {Ξ : proof_ctx n}
-                       {s : st},
-    wt_ctx Γ Ξ -> proving n Γ Ξ (𝕊 (𝕃ₛ s) []ₛ)
-| pr_sort_cons : forall {n : nat} {Γ : HOL_ctx n} {Ξ : proof_ctx n}
-                        {t u : tm n} {s : st},
-    proving n Γ Ξ (𝕊 s t) -> proving n Γ Ξ (𝕊 (𝕃ₛ s) u) ->
-    proving n Γ Ξ (𝕊 (𝕃ₛ s) (t ::ₛ u))
-| pr_sort_recL : forall {n : nat} {Γ : HOL_ctx n} {Ξ : proof_ctx n}
-                        {t u v : tm n} {s : st} (s' : st),
-    proving n Γ Ξ (𝕊 s t) -> proving n Γ Ξ (𝕊 (s' →ₛ 𝕃ₛ s' →ₛ s →ₛ s) u) ->
-    proving n Γ Ξ (𝕊 (𝕃ₛ s') v) -> proving n Γ Ξ (𝕊 s (rec𝕃ₛ t u v))
-| pr_sort_lam : forall {n : nat} {Γ : HOL_ctx n} {Ξ : proof_ctx n}
-                       {t : tm (S n)} {s s' : st},
-    proving (S n) (s .: Γ) ((𝕊 s ⟦ var_zero ⟧ₛ) :: map (ren_tm shift) Ξ) (𝕊 s' t) ->
-    proving n Γ Ξ (𝕊 (s →ₛ s') (ƛ t))
-| pr_sort_app : forall {n : nat} {Γ : HOL_ctx n} {Ξ : proof_ctx n}
-                       {t u : tm n} (s : st) {s' : st},
-    proving n Γ Ξ (𝕊 (s →ₛ s') t) -> proving n Γ Ξ (𝕊 s u) ->
-    proving n Γ Ξ (𝕊 s' (t @ₛ u))
-| pr_sort_pair : forall {n : nat} {Γ : HOL_ctx n} {Ξ : proof_ctx n}
-                        {t u : tm n} {s s' : st},
-    proving n Γ Ξ (𝕊 s t) -> proving n Γ Ξ (𝕊 s' u) ->
-    proving n Γ Ξ (𝕊 (s ×ₛ s') ⟨ t , u ⟩ₛ)
-| pr_sort_proj1 : forall {n : nat} {Γ : HOL_ctx n} {Ξ : proof_ctx n}
-                         {t : tm n} {s : st} (s' : st),
-    proving n Γ Ξ (𝕊 (s ×ₛ s') t) -> proving n Γ Ξ (𝕊 s (π¹ₛ t))
-| pr_sort_proj2 : forall {n : nat} {Γ : HOL_ctx n} {Ξ : proof_ctx n}
-                         {t : tm n} (s : st) {s' : st},
-    proving n Γ Ξ (𝕊 (s ×ₛ s') t) -> proving n Γ Ξ (𝕊 s' (π²ₛ t)).
+Notation "Γ ∣ Ξ ⊢ᴴᴼᴸ φ" := (proof Γ Ξ φ) (at level 65).
 
-Notation "Γ ∣ Ξ ⊢| n | φ" := (proving n Γ Ξ φ) (at level 87).
-
-Lemma wt_proving :
-  forall (n : nat) (Γ : HOL_ctx n) (Ξ : proof_ctx n) (φ : tm n),
-    Γ ∣ Ξ ⊢| n | φ -> wt_ctx Γ Ξ /\ (Γ ⊢⟨ n ⟩ φ ~: ℙₛ).
+Lemma lift_proof :
+  forall (Γ₀ Δ Γ₁ : HOL_ctx) (Ξ : proof_ctx (Γ₀ ++ Γ₁)) (φ : Γ₀ ++ Γ₁ ⊢ₛ ℙₛ),
+    Γ₀ ++ Γ₁ ∣ Ξ ⊢ᴴᴼᴸ φ ->
+    Γ₀ ++ Δ ++ Γ₁ ∣ map (lift_tm Γ₀ Δ Γ₁ ℙₛ) Ξ ⊢ᴴᴼᴸ lift_tm Γ₀ Δ Γ₁ ℙₛ φ.
 Proof.
-  intros. induction H; try (split; [assumption | ]);
-    try (destruct IHproving as [HΞ IH]; split; [try assumption | try assumption]);
-    try (destruct IHproving1 as [HΞ IH1]; destruct IHproving2 as [_ IH2];
-         try destruct IHproving3 as [_ IH3];
-         split; [try assumption| try assumption]);
-    try (constructor; constructor; fail).
-  - apply (In_forall _ Ξ φ H H0).
-  - dependent destruction HΞ. apply HΞ.
-  - constructor; [| assumption]. inversion HΞ.
-    apply H2.
-  - dependent destruction IH1. apply IH1_2.
-  - eapply (map_forall_rev _
-              (fun x => s .: Γ ⊢⟨ S n ⟩ x ~: ℙₛ)
-              (ren_tm shift)).
-    intros a Ha.
-    eapply typ_weaken_rev.
-    apply Ha. apply HΞ.
-  - apply typ_forall. apply IH.
-  - apply (comp_typ_vec _ _ _ _ (s .: Γ)).
-    asimpl. intro f; case f eqn:e.
-    asimpl. apply typ_var. asimpl. apply H0.
-    dependent destruction IH. apply IH.
-  - constructor. apply (typ_app ℕₛ).
-    apply typ_weaken. dependent destruction IH1.
-    dependent destruction IH1_2. apply IH1_1.
-    constructor.
-  - constructor. apply (typ_app 𝔹ₛ).
-    apply typ_weaken. dependent destruction IH2.
-    dependent destruction IH2_2. apply IH2_1.
-    constructor.
-  - constructor. apply (typ_app (𝕃ₛ s)).
-    apply typ_weaken. dependent destruction IH2.
-    dependent destruction IH2.
-    dependent destruction IH2.
-    dependent destruction IH2_2.
-    dependent destruction IH2_2_2.
-    apply (typ_weaken_rev _ _ _ _ s0).
-    apply (typ_weaken_rev _ _ _ _ (𝕃ₛ s0)).
-    asimpl. apply IH2_1. constructor.
-  - constructor. dependent destruction IH.
-    constructor. apply IH.
-  - constructor. dependent destruction IH1.
-    dependent destruction IH2.
-    dependent destruction IH3.
-    constructor; assumption.
-  - dependent destruction IH1.
-    dependent destruction IH2.
-    dependent destruction IH3.
-    constructor. constructor; assumption.
-  - dependent destruction IH1.
-    dependent destruction IH2.
-    constructor. constructor; assumption.
-  - dependent destruction IH1.
-    dependent destruction IH2.
-    dependent destruction IH3.
-    constructor. apply (typ_recL s'); assumption.
-  - dependent destruction HΞ.
-    eapply (map_forall_rev _
-              (fun x => s .: Γ ⊢⟨ S n ⟩ x ~: ℙₛ)
-              (ren_tm shift)).
-    intros a Ha.
-    eapply typ_weaken_rev.
-    apply Ha.
-    apply HΞ.
-  - constructor. constructor.
-    dependent destruction IH.
-    apply IH.
-  - constructor.
-    dependent destruction IH1.
-    dependent destruction IH2.
-    apply (typ_app s); assumption.
-  - constructor.
-    dependent destruction IH1.
-    dependent destruction IH2.
-    constructor; assumption.
-  - constructor. dependent destruction IH.
-    apply (typ_proj1 s'). assumption.
-  - constructor. dependent destruction IH.
-    apply (typ_proj2 s). assumption.
-Qed.
+  intros. dependent induction H.
+  - admit.
+  - autorewrite with lift_tm.
+    apply pr_imp_i.
+    specialize (IHproof Γ₀ Γ₁ (φ0 :: Ξ) ψ). apply IHproof; reflexivity.
+  - apply (pr_imp_e (lift_tm Γ₀ Δ Γ₁ _ φ0)).
+    specialize (IHproof1 Γ₀ Γ₁ Ξ (φ0 ⇒ₛ φ)). apply IHproof1; reflexivity.
+    apply IHproof2; reflexivity.
+  - autorewrite with lift_tm. apply pr_fora_i.
+    specialize (IHproof (s :: Γ₀) Γ₁ (map (fun φ => φ ↑ₛ s) Ξ)).
+    rewrite map_map in IHproof.
+    rewrite map_map.
+    assert (map (fun x => lift_tm (s :: Γ₀) Δ Γ₁ ℙₛ (x ↑ₛ s)) Ξ =
+              map (fun x => lift_tm Γ₀ Δ Γ₁ ℙₛ x ↑ₛ s) Ξ).
+    apply map_ext. intro φ. admit.
+    rewrite <- H0. apply IHproof; reflexivity.
+  - specialize (IHproof Γ₀ Γ₁ Ξ (∀ₛ s φ0) JMeq_refl JMeq_refl JMeq_refl).
+    autorewrite with lift_tm in IHproof.
+    apply (pr_fora_e (lift_tm Γ₀ Δ Γ₁ s t)) in IHproof.
+    admit.
+  - admit.
+Admitted.
 
-Lemma ren_proof :
-  forall (n m : nat) (Γ : HOL_ctx n) (Δ : HOL_ctx m)
-         (Ξ : proof_ctx n) (φ : tm n) (ξ : fin n -> fin m),
-    (forall f, (ξ >> Δ) f = Γ f) ->
-    Γ ∣ Ξ ⊢| n | φ -> Δ ∣ map (ren_tm ξ) Ξ ⊢| m | ren_tm ξ φ.
-Proof.
-  intros; revert m Δ ξ H; induction H0; intros; simpl.
-  - apply pr_ax.
-    apply (map_forall _ _ (ren_tm ξ)
-             (fun x => typ_ren m n ξ Δ Γ x _ H1)).
-    apply H. apply (in_map (ren_tm ξ) Ξ φ H0).
-  - apply (ren_βeq n m φ ψ ξ) in H1.
-    apply (pr_transp (ren_tm ξ φ)).
-    apply IHproving. apply H2. apply (typ_ren _ _ ξ Δ Γ).
-    apply H2. apply H. apply H1.
-  - simpl; apply pr_abs. apply IHproving. apply H.
-  - simpl. specialize (IHproving1 _ _ _ H).
-    specialize (IHproving2 _ _ _ H).
-    apply (pr_app _ IHproving1 IHproving2).
-  - asimpl. apply pr_abs_f.
-    specialize (IHproving _ (s .: Δ) (var_zero .: ξ >> shift)).
-    asimpl in IHproving.
-    rewrite map_map in IHproving. asimpl in IHproving.
-    rewrite map_map. asimpl.
-    apply IHproving.
-    intro f. unfold ">>". asimpl.
-    case f eqn : e. simpl. asimpl. unfold ">>"; simpl.
-    apply H. unfold ">>"; simpl. reflexivity.
-  - simpl. asimpl.
-    specialize (IHproving m Δ ξ H1).
-    asimpl in IHproving.
-    assert (Δ ⊢⟨ m ⟩ ren_tm ξ t ~: s).
-    apply (typ_ren _ _ _ _ _ _ _ H1 H).
-    specialize (pr_app_f _ _ IHproving H2); intro.
-    asimpl in H3. apply H3.
-  - asimpl.
-    specialize (IHproving1 m Δ ξ H); specialize (IHproving2 m Δ ξ H).
-    asimpl in IHproving2.
-    specialize (@pr_recN m Δ (map (ren_tm ξ) Ξ) (ren_tm ξ φ) IHproving1).
-    intro H0. asimpl in H0. apply H0.
-    apply IHproving2.
-  - asimpl.
-    specialize (IHproving1 m Δ ξ H).
-    specialize (IHproving2 m Δ ξ H).
-    asimpl in IHproving1; asimpl in IHproving2.
-    specialize (pr_recB IHproving1 IHproving2).
-    asimpl. trivial.
-  - asimpl.
-    specialize (IHproving1 m Δ ξ H).
-    specialize (IHproving2 m Δ ξ H).
-    asimpl in IHproving1; simpl in IHproving2.
-    specialize (@pr_recL m Δ (map (ren_tm ξ) Ξ) s (ren_tm ξ φ)).
-    asimpl. intro H0; specialize (H0 IHproving1).
-    apply H0.
-    unfold ">>" in IHproving2.
-    asimpl in IHproving2.
-    apply IHproving2.
-  - apply pr_sort_Z.
-    apply (map_forall (fun x => Γ ⊢⟨ n ⟩ x ~: ℙₛ)
-             (fun x => Δ ⊢⟨ m ⟩ x ~: ℙₛ)
-             (ren_tm ξ)).
-    intros a Ha.
-    eapply typ_ren.
-    apply H0. apply Ha.
-    apply H.
-  - apply pr_sort_S.
-    apply IHproving. apply H.
-  - apply pr_sort_recN.
-    apply IHproving1; assumption.
-    apply IHproving2; assumption.
-    apply IHproving3; assumption.
-  - apply pr_sort_T.
-    apply (map_forall (fun x => Γ ⊢⟨ n ⟩ x ~: ℙₛ)
-             (fun x => Δ ⊢⟨ m ⟩ x ~: ℙₛ)
-             (ren_tm ξ)).
-    intros a Ha.
-    eapply typ_ren.
-    apply H0. apply Ha.
-    apply H.
-  - apply pr_sort_F.
-    apply (map_forall (fun x => Γ ⊢⟨ n ⟩ x ~: ℙₛ)
-             (fun x => Δ ⊢⟨ m ⟩ x ~: ℙₛ)
-             (ren_tm ξ)).
-    intros a Ha.
-    eapply typ_ren.
-    apply H0. apply Ha.
-    apply H.
-  - apply pr_sort_recB.
-    apply IHproving1; assumption.
-    apply IHproving2; assumption.
-    apply IHproving3; assumption.
-  - apply pr_sort_nil.
-    apply (map_forall (fun x => Γ ⊢⟨ n ⟩ x ~: ℙₛ)
-             (fun x => Δ ⊢⟨ m ⟩ x ~: ℙₛ)
-             (ren_tm ξ)).
-    intros a Ha.
-    eapply typ_ren.
-    apply H0. apply Ha.
-    apply H.
-  - apply pr_sort_cons.
-    apply IHproving1; assumption.
-    apply IHproving2; assumption.
-  - apply (pr_sort_recL s').
-    apply IHproving1; assumption.
-    apply IHproving2; assumption.
-    apply IHproving3; assumption.
-  - apply pr_sort_lam.
-    specialize (IHproving (S m) (s .: Δ) (upRen_tm_tm ξ)).
-    asimpl in IHproving.
-    assert
-      (forall f, ((var_zero .: ξ >> shift) >> (s .: Δ)) f = (s .: Γ) f).
-    intro f; case f eqn : e. asimpl.
-    unfold ">>"; simpl. apply H. reflexivity.
-    specialize (IHproving H1); clear H1.
-    asimpl in IHproving. simpl in IHproving.
-    rewrite map_map in IHproving.
-    asimpl in IHproving.
-    rewrite map_map. asimpl.
-    assert (forall f,
-               (ren_tm shift >> ren_tm (var_zero .: ξ >> shift)) f =
-                 (ren_tm ξ >> ren_tm shift) f).
-    intro f; asimpl. reflexivity. apply IHproving.
-  - apply (pr_sort_app s).
-    apply IHproving1; assumption.
-    apply IHproving2; assumption.
-  - apply pr_sort_pair.
-    apply IHproving1; assumption.
-    apply IHproving2; assumption.
-  - apply (pr_sort_proj1 s').
-    apply IHproving; assumption.
-  - apply (pr_sort_proj2 s).
-    apply IHproving; assumption.
-Qed.
-
-Lemma subst_proof :
-  forall (n m : nat) (v : HOL_vec n m) (Γ : HOL_ctx m) (Δ : HOL_ctx n)
-         (Ξ : proof_ctx n) (φ : tm n),
-    Γ ⊢⟨ m ⟩ v ~:⟨ n , Δ ⟩ -> Δ ∣ Ξ ⊢| n | φ ->
-    Γ ∣ map (subst_tm v) Ξ ⊢| m | φ [ v ].
-Proof.
-  intros n m v Γ Δ Ξ φ Hv Hφ; revert m v Γ Hv; induction Hφ; intros; simpl.
-  - apply pr_ax.
-    apply (map_forall (fun x => Γ  ⊢⟨ n ⟩ x ~: ℙₛ)
-             (fun x => Γ0 ⊢⟨ m ⟩ x ~: ℙₛ)).
-    intro a. apply comp_typ_vec.
-    apply Hv. apply H.
-    apply (in_map (subst_tm v) Ξ φ H0).
-  - apply (subst_βeq n m φ ψ v) in H0.
-    apply (pr_transp (subst_tm v φ)).
-    apply IHHφ. apply Hv.
-    apply (comp_typ_vec _ _ v Γ0 Γ).
-    apply Hv. apply H. apply H0.
-  - asimpl. apply pr_abs. apply IHHφ.
-    apply Hv.
-  - specialize (IHHφ1 _ _ _ Hv).
-    specialize (IHHφ2 _ _ _ Hv).
-    apply (pr_app _ IHHφ1 IHHφ2).
-  - asimpl. apply pr_abs_f.
-    specialize (IHHφ (S m) ((S m)__tm var_zero .: v >> ren_tm shift)
-                  (s .: Γ0)).
-    asimpl in IHHφ.
-    assert (s .: Γ0 ⊢⟨ S m ⟩ (S m)__tm var_zero .: v >> ren_tm shift ~:⟨ S n, s .: Γ ⟩).
-    intro f. case f eqn : e.
-    asimpl. unfold ">>". apply typ_weaken. apply Hv.
-    constructor.
-    specialize (IHHφ H).
-    assert (map (subst_tm ((S m)__tm var_zero .: v >> ren_tm shift)) (map (ren_tm shift) Ξ) =
-              (map (ren_tm shift) (map (subst_tm v) Ξ))).
-    rewrite map_map. asimpl. unfold ">>". rewrite map_map. apply map_ext.
-    intro f. asimpl. reflexivity.
-    rewrite <- H0. apply IHHφ.
-  - asimpl. specialize (IHHφ m v Γ0 Hv).
-    asimpl in IHHφ.
-    apply (@pr_app_f _ _ _ _ (t [v])) in IHHφ.
-    asimpl in IHHφ.
-    assert (φ [t[v] .: v >> (ren_tm shift >> subst_tm (t[v] .: m __tm))] = φ[t[v] .: v]).
-    apply ext_tm.
-    intro f; case f eqn : e.
-    asimpl. reflexivity. reflexivity.
-    apply (eq_rec _ (proving m Γ0 (map (subst_tm v) Ξ)) IHHφ _ H0).
-    apply (comp_typ_vec _ _ _ _ _ _ _ Hv H).
-  - specialize (IHHφ1 m v Γ0 Hv). specialize (IHHφ2 m v Γ0 Hv).
-    asimpl. asimpl in IHHφ1. asimpl in IHHφ2.
-    assert (subst_tm (v >> ren_tm shift) φ = ren_tm shift (subst_tm v φ)).
-    asimpl. reflexivity.
-    rewrite H in IHHφ2.
-    specialize (pr_recN IHHφ1 IHHφ2).
-    asimpl. trivial.
-  - asimpl; asimpl in IHHφ1; asimpl in IHHφ2.
-    specialize (pr_recB (IHHφ1 _ _ _ Hv) (IHHφ2 _ _ _ Hv)).
-    asimpl. trivial.
-  - specialize (IHHφ1 m v Γ0 Hv); specialize (IHHφ2 m v Γ0 Hv).
-    asimpl; asimpl in IHHφ1; asimpl in IHHφ2.
-    assert
-      (subst_tm
-         (shift >>
-            (((S m)__tm var_zero .: v >> ren_tm shift) >>
-               ren_tm shift)) φ =
-         ren_tm (shift >> shift) (subst_tm v φ)).
-    asimpl. apply ext_tm.
-    intro; unfold ">>"; asimpl.
-    reflexivity.
-    rewrite H in IHHφ2; clear H.
-    specialize (pr_recL IHHφ1 IHHφ2).
-    asimpl. trivial.
-  - apply pr_sort_Z.
-    apply (map_forall
-             (fun x => Γ  ⊢⟨ n ⟩ x ~: ℙₛ)
-             (fun x => Γ0 ⊢⟨ m ⟩ x ~: ℙₛ)
-             (subst_tm v)).
-    intros a Ha.
-    apply (comp_typ_vec _ _ _ _ _ _ _ Hv Ha).
-    apply H.
-  - asimpl. apply pr_sort_S.
-    apply IHHφ.
-    apply Hv.
-  - asimpl. apply pr_sort_recN.
-    apply IHHφ1; assumption.
-    apply IHHφ2; assumption.
-    apply IHHφ3; assumption.
-  - apply pr_sort_T.
-    apply (map_forall
-             (fun x => Γ  ⊢⟨ n ⟩ x ~: ℙₛ)
-             (fun x => Γ0 ⊢⟨ m ⟩ x ~: ℙₛ)
-             (subst_tm v)).
-    intros a Ha.
-    apply (comp_typ_vec _ _ _ _ _ _ _ Hv Ha).
-    apply H.
-  - apply pr_sort_F.
-    apply (map_forall
-             (fun x => Γ  ⊢⟨ n ⟩ x ~: ℙₛ)
-             (fun x => Γ0 ⊢⟨ m ⟩ x ~: ℙₛ)
-             (subst_tm v)).
-    intros a Ha.
-    apply (comp_typ_vec _ _ _ _ _ _ _ Hv Ha).
-    apply H.
-  - asimpl. apply pr_sort_recB.
-    apply IHHφ1; assumption.
-    apply IHHφ2; assumption.
-    apply IHHφ3; assumption.
-  - apply pr_sort_nil.
-    apply (map_forall
-             (fun x => Γ  ⊢⟨ n ⟩ x ~: ℙₛ)
-             (fun x => Γ0 ⊢⟨ m ⟩ x ~: ℙₛ)
-             (subst_tm v)).
-    intros a Ha.
-    apply (comp_typ_vec _ _ _ _ _ _ _ Hv Ha).
-    apply H.
-  - asimpl. apply pr_sort_cons.
-    apply IHHφ1; assumption.
-    apply IHHφ2; assumption.
-  - asimpl. apply (pr_sort_recL s').
-    apply IHHφ1; assumption.
-    apply IHHφ2; assumption.
-    apply IHHφ3; assumption.
-  - asimpl. apply pr_sort_lam.
-    specialize (IHHφ (S m) ((S m)__tm var_zero .: v >> ren_tm shift)
-                  (s .: Γ0)).
-    assert (s .: Γ0 ⊢⟨ S m ⟩ (S m) __tm var_zero .: v >> ren_tm shift ~:⟨ S n, s .: Γ ⟩).
-    intro f. case f eqn : e.
-    asimpl. unfold ">>". apply typ_weaken. apply Hv.
-    asimpl. constructor.
-    specialize (IHHφ H); clear H.
-    asimpl in IHHφ.
-    rewrite map_map. asimpl.
-    simpl in IHHφ. rewrite map_map in IHHφ.
-    asimpl in IHHφ.
-    assert
-      (forall f,
-          (ren_tm shift >> subst_tm
-             ((S m)__tm var_zero .: v >> ren_tm shift)) f =
-            (subst_tm v >> ren_tm shift) f).
-    intro f; asimpl. reflexivity.
-    apply IHHφ.
-  - asimpl. apply (pr_sort_app s).
-    apply IHHφ1; assumption.
-    apply IHHφ2; assumption.
-  - asimpl. apply pr_sort_pair.
-    apply IHHφ1; assumption.
-    apply IHHφ2; assumption.
-  - asimpl. apply (pr_sort_proj1 s').
-    apply IHHφ; assumption.
-  - asimpl. apply (pr_sort_proj2 s).
-    apply IHHφ; assumption.
-Qed.
-
-Lemma weaken_proof :
-  forall (n : nat) (Γ : HOL_ctx n)
-         (Ξ Θ : proof_ctx n) (φ : tm n),
-    Γ ∣ Ξ ⊢| n | φ -> incl Ξ Θ ->
-    wt_ctx Γ Θ -> Γ ∣ Θ ⊢| n | φ.
-Proof.
-  intros; revert Θ H0 H1; induction H; intros.
-  - apply pr_ax. apply H2. apply H1.
-    apply H0.
-  - apply (pr_transp φ). apply IHproving.
-    apply H2. apply H3. apply H0. apply H1.
-  - apply pr_abs. apply IHproving.
-    intro χ. intro χφΞ.
-    simpl; simpl in χφΞ.
-    destruct χφΞ as [ φχ | χΞ ].
-    left; apply φχ.
-    right; apply (H0 _ χΞ).
-    constructor.
-    destruct (wt_proving n Γ (φ :: Ξ) ψ H) as [H2 _].
-    inversion H2. apply H5.
-    apply H1.
-  - apply (pr_app φ). apply IHproving1.
-    apply H1. apply H2. apply IHproving2.
-    apply H1. apply H2.
-  - apply pr_abs_f. apply IHproving.
-    intro x.
-    intro xΞ. rewrite in_map_iff. rewrite in_map_iff in xΞ.
-    destruct xΞ. exists x0. destruct H2.
-    split; [apply H2|].
-    apply H0. apply H3.
-    apply (map_forall _ _ (ren_tm shift)
-             (fun x => typ_weaken n Γ x _ _) Θ H1).
-  - apply (pr_app_f t s).
-    apply IHproving. apply H1. apply H2.
-    apply H0.
-  - apply pr_recN. apply IHproving1. apply H1. apply H2.
-    apply IHproving2. apply H1. apply H2.
-  - apply pr_recB. apply IHproving1. apply H1. apply H2.
-    apply IHproving2. apply H1. apply H2.
-  - apply pr_recL. apply IHproving1. apply H1. apply H2.
-    apply IHproving2. apply H1. apply H2.
-  - apply pr_sort_Z; assumption.
-  - apply pr_sort_S. apply IHproving; assumption.
-  - apply pr_sort_recN.
-    apply IHproving1; assumption.
-    apply IHproving2; assumption.
-    apply IHproving3; assumption.
-  - apply pr_sort_T; assumption.
-  - apply pr_sort_F; assumption.
-  - apply pr_sort_recB.
-    apply IHproving1; assumption.
-    apply IHproving2; assumption.
-    apply IHproving3; assumption.
-  - apply pr_sort_nil; assumption.
-  - apply pr_sort_cons.
-    apply IHproving1; assumption.
-    apply IHproving2; assumption.
-  - apply (pr_sort_recL s').
-    apply IHproving1; assumption.
-    apply IHproving2; assumption.
-    apply IHproving3; assumption.
-  - apply pr_sort_lam. apply IHproving.
-    apply incl_cons.
-    left; reflexivity.
-    apply incl_tl.
-    apply incl_map. apply H0.
-    constructor.
-    constructor. constructor.
-    apply (map_forall
-             (fun x => Γ  ⊢⟨ n ⟩ x ~: ℙₛ)
-             (fun x => s .: Γ ⊢⟨ S n ⟩ x ~: ℙₛ)
-             (ren_tm shift)).
-    intros a Ha. apply typ_weaken.
-    apply Ha.
-    apply H1.
-  - apply (pr_sort_app s).
-    apply IHproving1; assumption.
-    apply IHproving2; assumption.
-  - apply pr_sort_pair.
-    apply IHproving1; assumption.
-    apply IHproving2; assumption.
-  - apply (pr_sort_proj1 s').
-    apply IHproving; assumption.
-  - apply (pr_sort_proj2 s).
-    apply IHproving; assumption.
-Qed.
-
-Lemma weaken_proof_1 :
-  forall (n : nat) (Γ : HOL_ctx n)
-         (Ξ : proof_ctx n) (φ ψ : tm n),
-    Γ ∣ Ξ ⊢| n | φ -> Γ ⊢⟨ n ⟩ ψ ~: ℙₛ ->
-    Γ ∣ ψ :: Ξ ⊢| n | φ.
-Proof.
-  intros.
-  apply (weaken_proof n Γ Ξ (ψ :: Ξ)).
-  apply H. intros x xΞ; simpl; right; apply xΞ.
-  constructor. apply H0.
-  apply (wt_proving n Γ Ξ φ H).
-Qed.
